Simplify online secrecy (#16)
* Online with secrecy: use simplified key setup and explicit key session ids (matching the first model for the Online? protocol)

* rephrased Online? secrecy to more intuitive version

* NSL: simplifying properties

* online secrecy: hiding trace_invariant in property

* NSL: hiding trace_invariant from properties

dy-extensions/DY.Simplified.fst
@@ -12,6 +12,8 @@ let gen_rand =
 let gen_rand_labeled l =
     mk_rand NoUsage l 32
 
+let principal_is_corrupt tr prin = is_corrupt tr (principal_label prin)
+
 val start_new_session:
   #a:Type -> {| local_state a |} ->
   principal -> a ->
